casting to anybytes

bedrock2/src/bedrock2/SepLib.v
@@ -1,10 +1,9 @@
 Require Import Coq.ZArith.ZArith. Local Open Scope Z_scope.
 Require Import Coq.micromega.Lia.
-Require Import coqutil.Word.Interface.
-Require Import coqutil.Word.Bitwidth.
+Require Import coqutil.Word.Interface coqutil.Word.Properties coqutil.Word.Bitwidth.
 Require Import coqutil.Map.Interface.
 Require Import coqutil.Datatypes.ZList. Import ZList.List.ZIndexNotations.
-Require Import bedrock2.Map.Separation bedrock2.Map.SeparationLogic.
+Require Import bedrock2.Lift1Prop bedrock2.Map.Separation bedrock2.Map.SeparationLogic.
 Require Import bedrock2.PurifySep.
 Require Import bedrock2.Array bedrock2.Scalars.
 
@@ -116,18 +115,161 @@ Lemma purify_uintptr{width}{BW: Bitwidth width}{word: word width}
 Proof. unfold purify. intros. constructor. Qed.
 #[export] Hint Resolve purify_uintptr : purify.
 
+Section WithMem.
+  Context {width} {BW: Bitwidth width} {word: word width} {mem: map.map word Byte.byte}
+          {word_ok: word.ok word} {mem_ok: map.ok mem}.
 
-Definition anybytes{width}{BW: Bitwidth width}{word: word width}{mem: map.map word Byte.byte}
-  (sz: Z)(a: word)(m: mem): Prop := 0 <= sz /\ Memory.anybytes a sz m.
+  Definition anybytes(sz: Z)(a: word): mem -> Prop :=
+    ex1 (fun bytes => array (uint 8) sz bytes a).
+
+  Lemma purify_anybytes sz a:
+    purify (anybytes sz a) (0 <= sz).
+    (* Note:
+     - (sz <= 2^width) would hold (because of max memory size)
+     - (sz < 2^width) would be more useful but is not provable currently *)
+  Proof.
+    unfold purify, anybytes, ex1. intros * [bytes Hm].
+    eapply purify_array in Hm. lia.
+  Qed.
+
+  Lemma sep_assoc_eq: forall (p q r: mem -> Prop),
+      sep (sep p q) r = sep p (sep q r).
+  Proof.
+    intros. eapply iff1ToEq. eapply sep_assoc.
+  Qed.
+
+  (* The opposite direction does not hold because (len (vs1 ++ vs2) = n1 + n2) does
+     not imply (len vs1 = n1 /\ len vs2 = n2), but we can quantify over a vs:=vs1++vs2
+     and use vs[:i] ++ vs[i:], resulting in the lemma split_array below *)
+  Lemma merge_array{T: Type}(elem: T -> word -> mem -> Prop){sz: PredicateSize elem}:
+    forall n1 n2 vs1 vs2 a m,
+      sep (array elem n1 vs1 a)
+          (array elem n2 vs2 (word.add a (word.of_Z (sz * n1)))) m ->
+      array elem (n1 + n2) (vs1 ++ vs2) a m.
+  Proof.
+    unfold array. intros.
+    pose proof (Array.array_append (fun (a0 : word) (v : T) => elem v a0)
+                  (word.of_Z sz) vs1 vs2 a) as A.
+    eapply iff1ToEq in A.
+    rewrite A. clear A.
+    rewrite sep_assoc_eq in H.
+    eapply sep_emp_l in H.
+    destruct H as [? H]. subst n1.
+    eapply sep_comm in H.
+    rewrite sep_assoc_eq in H.
+    eapply sep_emp_l in H.
+    destruct H as [? H]. subst n2.
+    eapply sep_emp_l. split.
+    1: rewrite List.app_length; lia.
+    rewrite word.ring_morph_mul.
+    rewrite word.of_Z_unsigned.
+    rewrite <- word.ring_morph_mul.
+    eapply sep_comm in H.
+    exact H.
+  Qed.
+
+  Import ZList.List.ZIndexNotations.
+  Local Open Scope zlist_scope.
+
+  Lemma split_array{T: Type}(elem: T -> word -> mem -> Prop){sz: PredicateSize elem}:
+    forall vs n i a m,
+      0 <= i <= len vs ->
+      array elem n vs a m ->
+      sep (array elem i vs[:i] a)
+          (array elem (n-i) vs[i:] (word.add a (word.of_Z (sz * i)))) m.
+  Proof.
+    unfold array. intros.
+    eapply sep_emp_l in H0. destruct H0.
+    rewrite (List.split_at_index vs i) in H1 by assumption.
+    eapply Array.array_append in H1.
+    rewrite sep_assoc_eq.
+    eapply sep_emp_l.
+    split.
+    { apply List.len_upto. assumption. }
+    apply sep_comm.
+    rewrite sep_assoc_eq.
+    eapply sep_emp_l.
+    split.
+    { subst. apply List.len_from. assumption. }
+    rewrite word.ring_morph_mul in H1.
+    rewrite word.of_Z_unsigned in H1.
+    rewrite <- word.ring_morph_mul in H1.
+    rewrite List.len_upto in H1 by assumption.
+    apply sep_comm.
+    exact H1.
+  Qed.
+
+  Lemma merge_anybytes: forall n1 n2 addr m,
+      sep (anybytes n1 addr) (anybytes n2 (word.add addr (word.of_Z n1))) m ->
+      anybytes (n1 + n2) addr m.
+  Proof.
+    unfold anybytes. intros * Hm.
+    eapply sep_ex1_l in Hm. destruct Hm as [bs1 Hm].
+    eapply sep_ex1_r in Hm. destruct Hm as [bs2 Hm].
+    exists (bs1 ++ bs2).
+    eapply merge_array. rewrite Z.mul_1_l.
+    exact Hm.
+  Qed.
+
+  Lemma split_anybytes: forall n i addr m,
+      0 <= i <= n ->
+      anybytes n addr m ->
+      sep (anybytes i addr) (anybytes (n-i) (word.add addr (word.of_Z i))) m.
+  Proof.
+    intros * B Hm.
+    destruct Hm as [bs Hm].
+    pose proof Hm as HP. eapply purify_array in HP.
+    unfold anybytes.
+    eapply sep_ex1_l. exists bs[:i].
+    eapply sep_ex1_r. exists bs[i:].
+    subst n.
+    eapply split_array in Hm. 2: eassumption.
+    rewrite Z.mul_1_l in Hm.
+    exact Hm.
+  Qed.
+
+  Lemma ptsto_to_uint8: forall a b m, ptsto a b m -> uint 8 (Byte.byte.unsigned b) a m.
+  Proof.
+    intros a b m Hb.
+    eapply sep_emp_l. split. 1: eapply Byte.byte.unsigned_range.
+    unfold littleendian, ptsto_bytes.ptsto_bytes. simpl.
+    eapply sep_emp_True_r.
+    rewrite Byte.byte.of_Z_unsigned.
+    exact Hb.
+  Qed.
+
+  Lemma uint8_to_ptsto: forall a b m, uint 8 b a m -> ptsto a (Byte.byte.of_Z b) m.
+  Proof.
+    unfold uint. intros a b m Hb. eapply sep_emp_l in Hb. destruct Hb as (B & Hb).
+    unfold littleendian, ptsto_bytes.ptsto_bytes in Hb. simpl in Hb.
+    eapply sep_emp_True_r. exact Hb.
+  Qed.
+
+  Lemma anybytes_from_alt: forall addr n m,
+      0 <= n -> Memory.anybytes addr n m -> anybytes n addr m.
+  Proof.
+    unfold anybytes. intros * B H.
+    eapply anybytes_to_array_1 in H. destruct H as (bs & Hm & Hl).
+    exists (List.map Byte.byte.unsigned bs).
+    unfold array. eapply sep_emp_l. split.
+    { rewrite List.map_length. lia. }
+    eapply array_map.
+    eapply impl1_array. 2: exact Hm.
+    unfold impl1. eapply ptsto_to_uint8.
+  Qed.
+
+  Lemma anybytes_to_alt: forall addr n m,
+      anybytes n addr m -> Memory.anybytes addr n m.
+  Proof.
+    unfold anybytes. intros. destruct H as (bs & H).
+    unfold array in H. eapply sep_emp_l in H. destruct H as (? & H). subst n.
+    eapply impl1_array in H.
+    - eapply (array_map ptsto Byte.byte.of_Z addr bs (word.of_Z 1)) in H.
+      eapply array_1_to_anybytes in H. rewrite List.map_length in H. exact H.
+    - clear m bs addr H. unfold impl1. eapply uint8_to_ptsto.
+  Qed.
+End WithMem.
 
 #[export] Hint Extern 1 (PredicateSize (anybytes ?sz)) => exact sz
 : typeclass_instances.
-
-Lemma purify_anybytes{width}{BW: Bitwidth width}{word: word width}
-  {mem: map.map word Byte.byte} sz a:
-  purify (anybytes sz a) (0 <= sz).
-  (* Note:
-     - (sz <= 2^width) would hold (because of max memory size)
-     - (sz < 2^width) would be more useful but is not provable currently *)
-Proof. unfold purify, anybytes. intros * [? ?]. assumption. Qed.
 #[export] Hint Resolve purify_anybytes : purify.
