bedrock2/src/bedrock2/to_from_anybytes.v
@@ -1,0 +1,97 @@
+Require Import Coq.ZArith.ZArith. Local Open Scope Z_scope.
+Require Import Coq.micromega.Lia.
+Require Import coqutil.Word.Interface coqutil.Word.Properties coqutil.Word.Bitwidth.
+Require Import coqutil.Map.Interface.
+Require Import coqutil.Datatypes.ZList. Import ZList.List.ZIndexNotations.
+Require Import bedrock2.Lift1Prop bedrock2.Map.Separation bedrock2.Map.SeparationLogic.
+Require Import bedrock2.SepLib.
+Require Import bedrock2.sepapp.
+
+Section WithMem.
+  Context {width} {BW: Bitwidth width} {word: word width} {mem: map.map word Byte.byte}
+          {word_ok: word.ok word} {mem_ok: map.ok mem}.
+
+  Definition contiguous(P: word -> mem -> Prop)(n: Z): Prop :=
+    forall addr, impl1 (P addr) (anybytes n addr).
+
+  Lemma cast_to_anybytes: forall (P: word -> mem -> Prop) a n m,
+      contiguous P n -> P a m -> anybytes n a m.
+  Proof. unfold contiguous, impl1. intros. eauto. Qed.
+
+  (* the direction we care about is anybytes -> P, but it is very likely to
+     also imply the converse direction, and probably also easy to prove,
+     so we make it an iff1 *)
+  Definition fillable{V: Type}(P: V -> word -> mem -> Prop)(n: Z): Prop :=
+    forall addr, iff1 (anybytes n addr) (ex1 (fun v => P v addr)).
+
+  Lemma fillable_to_contiguous{V: Type} P (v: V) n: fillable P n -> contiguous (P v) n.
+  Proof.
+    unfold fillable, contiguous. intros. specialize (H addr).
+    unfold ex1, impl1 in *.
+    intros m Hm.
+    eapply proj2 in H.
+    eapply H.
+    eauto.
+  Qed.
+
+  Lemma anybytes_contiguous: forall n, contiguous (anybytes n) n.
+  Proof. unfold contiguous. intros. reflexivity. Qed.
+
+  Lemma sepapps_nil_contiguous: contiguous (sepapps nil) 0.
+  Proof.
+    unfold contiguous, sepapps, anybytes, Memory.anybytes, impl1.
+    simpl. intros *. intros [? _]. subst.
+    exists nil. unfold array.
+    eapply sep_emp_l. split; [reflexivity| ].
+    simpl. unfold emp. auto.
+  Qed.
+
+  Lemma sepapps_cons_contiguous: forall p tail n1 n2,
+      contiguous p n1 ->
+      contiguous (sepapps tail) n2 ->
+      contiguous (sepapps (cons (mk_sized_predicate p n1) tail)) (n1 + n2).
+  Proof.
+    unfold contiguous. intros.
+    rewrite sepapps_cons.
+    simpl.
+    intros m Hm.
+    eapply merge_anybytes.
+    destruct Hm as (m1 & m2 & D & Hm1 & Hm2).
+    unfold impl1 in *.
+    exists m1, m2. eauto.
+  Qed.
+
+  Lemma uintptr_contiguous: forall v, contiguous (uintptr v) (Memory.bytes_per_word width).
+  Proof.
+    unfold contiguous, impl1, uintptr. intros.
+    eapply Scalars.scalar_to_anybytes in H.
+    eapply anybytes_from_alt.
+    1: destruct width_cases as [E|E]; rewrite E; cbv; discriminate.
+    assumption.
+  Qed.
+End WithMem.
+
+Section WithMem32.
+  Context {word: word 32} {BW: Bitwidth 32} {mem: map.map word Byte.byte}
+          {word_ok: word.ok word} {mem_ok: map.ok mem}.
+
+  Lemma uintptr32_contiguous: forall v, contiguous (uintptr v) 4.
+  Proof. eapply (uintptr_contiguous (width := 32)). Qed.
+End WithMem32.
+
+Section WithMem64.
+  Context {word: word 64} {BW: Bitwidth 64} {mem: map.map word Byte.byte}
+          {word_ok: word.ok word} {mem_ok: map.ok mem}.
+
+  Lemma uintptr64_contiguous: forall v, contiguous (uintptr v) 8.
+  Proof. eapply (uintptr_contiguous (width := 64)). Qed.
+End WithMem64.
+
+Create HintDb contiguous.
+Hint Resolve
+  sepapps_cons_contiguous
+  sepapps_nil_contiguous
+  uintptr32_contiguous
+  uintptr64_contiguous
+  anybytes_contiguous
+: contiguous.
